\revhist{9/13/89, pss; 7/30/92, pss; 3/23/94, pss; 10/14/94, pss; 9/6/96, pss}

\Sect{}{}{\SectType{SpecialAssistance}}{

\AsItem{1}{TX-3d}
{Find the locations of the maximum and minima of the function:
 %
 \Eqn{}{y(x) = 5 x^3 - 2 x^2 - 3 x + 2.}
 %
 First, find \m{dy/dx} and set it equal to zero:
 %
 \Eqn{}{\dfrac{dy}{dx}=15x^2-4x-3=0}
 %
 or
 %
 \Eqn{}{(5x - 3)(3x + 1) = 0.}
 %
 Solving for the zeros, maxima or minima of the original function occur at:
 \m{x = 3/5; x = -1/3}.
 The corresponding values of \m{y} are found by inserting those \m{x} values into
 the original equation, e.g. at \m{x = 3/5}:
 %
 \Eqn{}{y=5\left(\dfrac{3}{5}\right)^3 - 2\left(\dfrac{3}{5}\right)^2 -
 3\left(\dfrac{3}{5}\right) + 2 = \dfrac{14}{25},}
 %
 while at \m{x = -1/3, y = 70/27}.
 To find whether these points are maxima or minima, calculate the second
 derivative:
 %
 \Eqn{}{\dfrac{d^2y}{dx^2}=30x-4,}
 %
 so at \m{x = 3/5},
 %
 \Eqn{}{30\left(\dfrac{3}{5}\right)-4=14>0.}
 %
 Thus a minimum occurs at \m{(3/5,14/25)}.
 At \m{x = -1/3}:
 %
 \Eqn{}{30\left(-\dfrac{1}{3}\right)-4=-14<0}
 %
 so a maximum occurs at \m{(-1/3,70/27)}.
}

\AsItem{2}{TX-2b}
{The binomial theorem states that
 %
 \Eqn{}{(c+d)^p=c^p+pc^{p-1}d+\dfrac{p(p-1)}{(1)(2)}c^{p-2}d^2
                +\dfrac{p(p-1)(p-2)}{(1)(2)(3)} c^{p-3}d^3+\ldots}
 %
 so the expression \m{a(x + \Delta x)^p} becomes
 \m{ax^p+apx^{p-1}\Delta x\,+  \ldots +a\Delta x^p}.
 After subtracting \m{ax^p} and dividing by \m{\Delta x}, the only term that
 doesn't contain a factor of \m{\Delta x} is \m{apx^{p-1}}, so when the limit as
 \m{\Delta x\rightarrow 0} is taken, this is the  only non-zero term.
}

\AsItem{3}{TX-2f}
{Applying the trigonometric identity for \m{\sin A - \sin B}, where
 \m{A = kx + k \Delta x + \delta} and \m{B = kx + \delta}, we obtain:
 %
 \Eqn{}{\sin(kx+k\Delta x + \delta) - \sin(kx+\delta)=
             2\sin\left(\dfrac{k\Delta x}{2}\right)
             \cos\left(kx+\delta + \dfrac{k\Delta x}{2}\right).}
 %
 After dividing this express by \m{\Delta x} and taking the limit as
 \m{\Delta x \rightarrow 0}, we get:
 %
 \Eqn{}{\dfrac{dy(x)}{dx}=\lim_{\Delta x \rightarrow 0}
        k\left(\dfrac{\sin\left(\dfrac{k\Delta x}{2}\right)}
       {k\dfrac{\Delta x}{2}}\right)\cos(kx+\delta+\dfrac{k\Delta x}{2}).}
 %
}

\AsItem{4}{PS-problem~19}
{Set \m{z \equiv kr} so the integral becomes:
 %
 \Eqn{}{I = \dfrac{A}{k^2} \int z e^z\,dz\,.}
 %
 Now use the general form of integration by parts:
 %
 \Eqn{}{I = \int f \dfrac{dg}{dx}\,dx = f \,g - \int g \dfrac{df}{dx}\,dx\,.}
 %
 Comparing, we see that we should take:
 %
 \Eqn{}{f = z  \qquad and \qquad g = e^z\,,}
 %
 where we have used: \m{d(e^z)/dz = e^z}.
}

\AsItem{5}{TX-2e}
{The symbols used to express the chain rule in Sect.\,2e are already used in other ways in this problem,
 so we make the substitutions \m{f \rightarrow F}, \m{x \rightarrow g}, and then \m{t \rightarrow x}
 to get an equivalent chain rule:
 %
 \Eqn{}{\dfrac{dF(g(x))}{dx}= \left(\dfrac{dF}{dg}\right)\left(\dfrac{dg}{dx}\right)\,.}
 %
 Comparing the left side to the desired derivative, we make the correspondence:
 %
 \Eqn{}{g(x) = ax^2 + bx + c, \quad \text{so: } F(g) = g^{1/2}\,.}
 %
 Then the chain rule gives:
 %
 \Eqn{}{\dfrac{dF}{dx} = \left(\dfrac{1}{2}g^{-1/2}\right) (2ax +b) = \dfrac{2ax+b}{2(ax^2 +bx+c)^{1/2}}\,.}
 %
 }

\AsItem{6}{PS-14b}
{Define \m{z \equiv 5y}, so \m{dz = 5dy} hence \m{dy = (1/5) dz} and:
%
\Eqn{}{\int_0^\infty e^{-5y}\,dy = \dfrac{1}{5} \int^\infty_0 e^{-z}\,dz = \dfrac{1}{5} (1)\,.}
%
}

\AsItem{7}{PS-14c}
{Define \m{z \equiv \cos \theta} giving \m{dz = -(\sin \theta)\,d\theta} hence \m{(\sin\theta\,d\theta) \equiv -z\,dz},
 where \m{\theta = 0} is the same as  \m{z = 1}, and where \m{\theta = \pi/2} is the same as \m{z = 0}.
 Then:
 %
 \Eqn{}{\int_0^{\pi /2}\,\cos\theta\;\sin\theta\,d\theta = -\int_1^0 z\,dz = \int_0^1 z\,dz\,.}
%
}

\AsItem{7}{PS-20c}
{The slope of the function has a zero at \m{x = 0} and another at \m{x = -(2B)/(3A)}.
 The signs of the second derivatives show the first to be a maximum and the second a minimum.
 So just set \m{(1/3) = -(2B)/(3A)}.
}

}% /Sect
